generational_gc.md
@@ -1,0 +1,8 @@
+Extend the current mark and sweep garbage collector with a generation, copying collector, a la OCaml. The details of the OCaml GC can be found in https://dev.realworldocaml.org/garbage-collector.html. In particular, all the small allocations go into the fixed-sized minor heap first. Large allocations directly go into the major heap. Once the minor heap is full, do a minor collection that does a copying collection to the major heap. You will use the major heap allocation function for this. The combined GC should still preserve the abstract GC correctness. As a reference, you may want to look at what the sequential OCaml 4 runtime system does: https://github.com/ocaml/ocaml/tree/4.14.
+
+I want a full implementation of a generational collector as described above in
+GC.Impl.fst/fsti, but with the same end-to-end correctness theorem, i.e.,
+full_gc_correctness. We have to update both the allocator and the collector,
+parameterizing them by the size of large objects and the size of the minor and
+major heaps. We will reuse our existing coalescing ark-and-sweep collector for
+the major heap.
